Fp/Packing.lean
@@ -1,6 +1,41 @@
 import Fp.Basic
 
 @[bv_normalize]
+def PackedFloat.unpackNormOrNonzeroSubnorm (pf : PackedFloat e s) :
+  UnpackedFloat (exponentWidth e s) (s + 1) :=
+  if pf.isNorm then
+    {
+      sign := pf.sign
+      -- We cannot use `BitVec.signExtend` here because `pf.ex` is not in 2's complement representation.
+      -- It should be safe to use `setWidth'`
+      ex := pf.ex.zeroExtend _ - BitVec.ofNat _ (bias e) -- e - bias, but no adjustment for significand?
+      sig := pf.sig.cons true
+      : UnpackedFloat _ _
+    }
+  else -- bif pf.isSubnorm then
+    {
+      sign := pf.sign
+      ex := BitVec.ofInt _ (minNormalExp e)
+      sig := pf.sig.cons false
+      : UnpackedFloat _ _
+    }.normalize
+
+/--
+If we start with a packedFloat whose 'isZero' predicate says 'false',
+then we know that the unpacked version of it is also not zero. This is a useful fact to have when we want to rewrite
+-/
+@[simp, grind! →]
+axiom PackedFloat.unpackNormOrNonzeroSubnorm_isZero_eq_of_not_isZero (pf : PackedFloat e s) (hpf : ¬ pf.isZero := by grind) :
+  pf.unpackNormOrNonzeroSubnorm.isZero = false
+
+@[simp]
+theorem PackedFloat.sign_unpackNormOrNonzeroSubnorm_eq_sign (pf : PackedFloat e s) :
+    pf.unpackNormOrNonzeroSubnorm.sign = pf.sign := by
+  simp [PackedFloat.unpackNormOrNonzeroSubnorm]
+  by_cases hpf : pf.isNorm <;> simp [hpf]
+
+
+@[bv_normalize]
 def PackedFloat.unpack (pf : PackedFloat e s)
   : EUnpackedFloat (exponentWidth e s) (s + 1) :=
   bif pf.isNaN then
@@ -9,22 +44,37 @@ def PackedFloat.unpack (pf : PackedFloat e s)
     EUnpackedFloat.mkInfinity pf.sign
   else bif pf.isZero then
     EUnpackedFloat.mkZero pf.sign
-  else bif pf.isNorm then
-    ({
-      sign := pf.sign
-      -- We cannot use `BitVec.signExtend` here because `pf.ex` is not in 2's complement representation.
-      -- It should be safe to use `setWidth'`
-      ex := pf.ex.zeroExtend _ - BitVec.ofNat _ (bias e) -- e - bias, but no adjustment for significand?
-      sig := pf.sig.cons true
-      : UnpackedFloat _ _
-    }).toEUnpackedFloat
-  else -- bif pf.isSubnorm then
-    ({
-      sign := pf.sign
-      ex := BitVec.ofInt _ (minNormalExp e)
-      sig := pf.sig.cons false
-      : UnpackedFloat _ _
-    }).normalize.toEUnpackedFloat
+  else EUnpackedFloat.mkNumber (pf.unpackNormOrNonzeroSubnorm)
+
+@[simp, grind! .]
+theorem PackedFloat.isNaN_unpack_eq_isNaN (pf : PackedFloat e s) :
+    pf.unpack.isNaN = pf.isNaN := by
+  simp [PackedFloat.unpack]
+  by_cases hpf : pf.isNaN <;> simp [hpf]
+  · by_cases hinf : pf.isInfinite <;> simp [hinf]
+    · by_cases hzero : pf.isZero <;> simp [hzero]
+
+@[simp, grind! .]
+theorem PackedFloat.isInfinite_unpack_eq_isInfinite (pf : PackedFloat e s) :
+    pf.unpack.isInfinite = pf.isInfinite := by
+  simp [PackedFloat.unpack]
+  by_cases hnan : pf.isNaN <;> simp [hnan]
+  by_cases hpf : pf.isInfinite <;> simp [hpf]
+  · grind
+  · by_cases hinf : pf.isInfinite <;> simp [hinf]
+    · by_cases hzero : pf.isZero <;> simp [hzero]
+
+@[simp, grind! .]
+theorem PackedFloat.isZero_unpack_eq_isZero (pf : PackedFloat e s) :
+    pf.unpack.isZero = pf.isZero := by
+  simp [PackedFloat.unpack]
+  by_cases hnan : pf.isNaN <;> simp [hnan]
+  · grind
+  · by_cases hinf : pf.isInfinite <;> simp [hinf]
+    · grind
+    · by_cases hzero : pf.isZero <;> simp [hzero]
+
+
 
 @[bv_normalize]
 def EUnpackedFloat.pack (uf : EUnpackedFloat (exponentWidth e s) (s + 1))
@@ -53,30 +103,88 @@ def EUnpackedFloat.pack (uf : EUnpackedFloat (exponentWidth e s) (s + 1))
             (uf.sig >>> shift).truncate s
   }
 
+
 attribute [bv_normalize] BitVec.zero
 
-theorem PackedFloat.isInfinite_pack_unpack (pf : PackedFloat 5 10) (hpf : pf.unpack.isInfinite) :
+@[simp]
+theorem PackedFloat.unpack_eq_mkNumber_of_isNormOrNonzeroSubnorm
+  {pf : PackedFloat e s} (hpf : pf.isNormOrNonzeroSubnorm) :
+    pf.unpack = EUnpackedFloat.mkNumber pf.unpackNormOrNonzeroSubnorm := by
+  have hnan : ¬ pf.isNaN := by grind
+  have hinf : ¬ pf.isInfinite := by grind
+  have hzero : ¬ pf.isZero := by grind
+  simp [PackedFloat.unpack, hnan, hinf, hzero]
+
+@[simp, grind →]
+theorem PackedFloat.unpack_eq_NaN_of_isNaN (pf : PackedFloat e s) (hpf : pf.isNaN) :
+    pf.unpack = EUnpackedFloat.mkNaN := by
+  simp [PackedFloat.unpack, hpf]
+
+@[simp]
+theorem EUnpackedFloat.mkNaN_pack_eq_mkNaN : (EUnpackedFloat.mkNaN : EUnpackedFloat _ _).pack =
+  (PackedFloat.mkNaN : PackedFloat e s) := rfl
+
+@[simp]
+theorem EUnpackedFloat.mkInfinity_pack_eq_getInfinity (sign : Bool) :
+    (EUnpackedFloat.mkInfinity sign).pack = PackedFloat.getInfinity e s sign := by
+  simp [pack, PackedFloat.getInfinity]
+
+@[simp]
+theorem EUnpackedFloat.mkZero_pack_eq_getZero (sign : Bool) :
+    (EUnpackedFloat.mkZero sign).pack = PackedFloat.getZero e s sign := by
+  simp [pack, PackedFloat.getZero]
+
+@[simp, grind! .]
+theorem PackedFloat.unpack_getInfinity {sign : Bool}   :
+    (PackedFloat.getInfinity e s sign).unpack = if (0 < s) then EUnpackedFloat.mkInfinity sign else EUnpackedFloat.mkNaN  := by
+  simp [PackedFloat.unpack]
+  by_cases hs : 0 < s
+  · simp [hs]
+  · simp [hs]
+
+@[simp]
+theorem PackedFloat.unpack_eq_mkZero_of_isZero (pf : PackedFloat e s) (hpf : pf.isZero) :
+    pf.unpack = EUnpackedFloat.mkZero pf.sign := by
+  simp [PackedFloat.unpack, hpf]
+  grind
+
+@[simp]
+theorem PackedFloat.unpack_getZero {sign : Bool} :
+    (PackedFloat.getZero e s sign).unpack =
+      if 0 < e then EUnpackedFloat.mkZero sign else
+      if s = 0 then EUnpackedFloat.mkNaN else EUnpackedFloat.mkInfinity sign := by
+  by_cases he : 0 < e
+  · simp [he]
+  · simp [he]
+    simp [PackedFloat.unpack]
+    simp [show (e = 0) = true by grind]
+    by_cases hs : s = 0
+    · simp [hs]
+    · simp [hs]
+
+private theorem PackedFloat.isInfinite_pack_unpack_example (pf : PackedFloat 5 10) (hpf : pf.unpack.isInfinite) :
     pf.unpack.pack.isInfinite = pf.isInfinite ∧ pf.unpack.pack.sign = pf.sign := by
   bv_decide
 
-theorem PackedFloat.isNaN_pack_unpack (pf : PackedFloat 5 10) :
+
+private theorem PackedFloat.isNaN_pack_unpack_example (pf : PackedFloat 5 10) :
     pf.unpack.pack.isNaN = pf.isNaN := by
   bv_decide
 
-theorem PackedFloat.pack_unpack (pf : PackedFloat 5 10) (hpf : pf.isNormOrSubnorm) :
+private theorem PackedFloat.pack_unpack_example (pf : PackedFloat 5 10) (hpf : pf.isNormOrNonzeroSubnorm) :
     pf.unpack.pack = pf := by
   bv_decide
 
 
-theorem PackedFloat.pack_unpack_e0m1 (pf : PackedFloat 0 1) (hpf : pf.isNormOrSubnorm) :
+private theorem PackedFloat.pack_unpack_e0m1_example (pf : PackedFloat 0 1) (hpf : pf.isNormOrNonzeroSubnorm) :
     pf.unpack.pack = pf := by
   bv_decide
 
-theorem PackedFloat.pack_unpack_e1m0 (pf : PackedFloat 1 0) (hpf : pf.isNormOrSubnorm) :
+private theorem PackedFloat.pack_unpack_e1m0_example (pf : PackedFloat 1 0) (hpf : pf.isNormOrNonzeroSubnorm) :
     pf.unpack.pack = pf := by
   bv_decide
 
-example (pf : PackedFloat 0 0) (hpf : pf.isNormOrSubnorm) :
+example (pf : PackedFloat 0 0) (hpf : pf.isNormOrNonzeroSubnorm) :
     pf.isNaN = true := by
   bv_decide
 
