Fp/Theorems/SmtLibSemanticsQ.lean
@@ -4,6 +4,18 @@ This will be where our proofs of correctness will be written against.
 -/
 import Fp.SmtLibSemantics
 
+namespace Fp
+namespace SmtLibSemanticsQ
 
-namespace Rounding
-end Rounding
+/--
+The noncomputable implementation of rounding, that rounds an unpacked float of 'ein, sin'
+into a packed float of 'eout, sout' according to the SMT-Lib semantics.
+
+Our proofs will be against this definition.
+-/
+noncomputable abbrev smtLibRoundMethodQ (eout sout : Nat) : SmtLibSemantics.RoundMethod (PackedFloat eout sout) ExtRat :=
+  SmtLibSemantics.smtLibRoundMethod eout sout (R := ExtRat) (SmtLibSemantics.smtLibV) (SmtLibSemantics.smtLibV)
+
+end SmtLibSemanticsQ
+
+end Fp
