Fp.lean
@@ -11,3 +11,4 @@ import Fp.Sqrt
 import Fp.Subtraction
 import Fp.SmtLibSemantics
 -- import Fp.Proofs
+import Fp.Theorems
