Fp/Grind.lean
@@ -1,3 +1,28 @@
+namespace Fp
+
+attribute [simp] Rat.not_lt
+
+attribute [grind] Rat.pow_pos
+attribute [grind] Rat.pow_nonneg
+attribute [grind] Rat.le_of_lt
+attribute [grind] Rat.mul_nonneg
+attribute [grind] Rat.inv_pos
+-- attribute [grind] Rat.zpow_pos
+-- attribute [simp] Rat.inv_inv
+
+attribute [grind →] Rat.mul_pos
+
+
+@[grind ., grind →] -- I may also want grind → to know that a ⁻¹ is positive when a is positive.
+theorem Rat.inv_nonneg {a : Rat} (ha : 0 ≤ a) : 0 ≤ a⁻¹ := by
+  by_cases ha0 : a = 0 <;> grind
+
+@[grind .]
+theorem Rat.div_nonneg (a b : Rat) (hb : 0 ≤ b) (ha : 0 ≤ a) : 0 ≤ a / b := by grind
+
+@[grind .]
+theorem Rat.two_pow_pos (n : Int) : 0 < (2 : Rat) ^ n := by exact Rat.zpow_pos rfl
+
 @[grind =]
 theorem Int.toNat_neg_eq_zero_of_nonpos {z : Int} (h : z ≤ 0) : z.toNat = 0 := by
   grind
@@ -61,7 +86,7 @@ theorem Nat.lt_mul_of_lt_of_pos {a b c : Nat} (hab : a < b) (hc : 0 < c) :
 
 
 /- # Grind sets for power of two reasoning. -/
-@[grind! .]
+-- @[grind! .]
 theorem Nat.lt_two_pow_of_lt_two_pow_of_le {a n m : Nat}
     (ha : a < 2 ^ n := by grind) (hnm : n ≤ m := by grind) : a < 2 ^ m := by
   apply Nat.lt_of_lt_of_le
@@ -83,3 +108,5 @@ theorem Nat.two_pow_le_two_pow_of_le {n m : Nat}
   · omega
 
 attribute [grind =, grind =_] Nat.shiftLeft_eq
+
+end Fp
