Fp/Theorems/UnpackedRound.lean
@@ -1,0 +1,240 @@
+import Fp.UnpackedRound
+import Fp.SmtLibSemantics
+import Fp.Theorems.SmtLibSemanticsQ
+import Fp.Multiplication
+import Fp.Theorems.Packing
+
+namespace Fp
+
+@[simp]
+theorem roundQ_eq (eout sout : Nat) (rm : RoundingMode) (sign : Bool) (r : ExtRat):
+    (Fp.SmtLibSemanticsQ.smtLibRoundMethodQ eout sout).round rm sign r =
+    (SmtLibSemantics.smtLibRoundMethod eout sout
+      SmtLibSemantics.smtLibV SmtLibSemantics.smtLibV).round rm sign
+    r := rfl
+
+@[simp]
+theorem lower_NaN_eq_PackedFloat_mkNaN :
+  SmtLibSemantics.smtLibLower.lower ExtRat.NaN = (PackedFloat.mkNaN : PackedFloat e s) := sorry
+
+@[simp]
+theorem upper_NaN_eq_PackedFloat_mkNaN :
+  SmtLibSemantics.smtLibUpper.upper ExtRat.NaN = (PackedFloat.mkNaN : PackedFloat e s) := sorry
+
+@[simp]
+theorem roundRNA_mkNaN (eout sout : Nat) (sign : Bool) :
+  (SmtLibSemantics.smtLibRoundMethod eout sout SmtLibSemantics.smtLibV SmtLibSemantics.smtLibV).roundRNA sign
+    (ExtRat.NaN) = PackedFloat.mkNaN := by
+  simp [SmtLibSemantics.RoundMethod.roundRNA]
+
+@[simp]
+theorem roundRNE_mkNaN (eout sout : Nat) (sign : Bool) :
+  (SmtLibSemantics.smtLibRoundMethod eout sout SmtLibSemantics.smtLibV SmtLibSemantics.smtLibV).roundRNE sign
+    (ExtRat.NaN) = PackedFloat.mkNaN := by
+  simp [SmtLibSemantics.RoundMethod.roundRNE]
+
+@[simp]
+theorem roundRTP_mkNaN (eout sout : Nat) (sign : Bool) :
+  (SmtLibSemantics.smtLibRoundMethod eout sout SmtLibSemantics.smtLibV SmtLibSemantics.smtLibV).roundRTP sign
+    (ExtRat.NaN) = PackedFloat.mkNaN := by
+  simp [SmtLibSemantics.RoundMethod.roundRTP]
+
+@[simp]
+theorem roundRTN_mkNaN (eout sout : Nat) (sign : Bool) :
+  (SmtLibSemantics.smtLibRoundMethod eout sout SmtLibSemantics.smtLibV SmtLibSemantics.smtLibV).roundRTN sign
+    (ExtRat.NaN) = PackedFloat.mkNaN := by
+  simp [SmtLibSemantics.RoundMethod.roundRTN]
+  rcases sign <;> simp
+
+@[simp]
+theorem rountRTZ_mkNaN (eout sout : Nat) (sign : Bool) :
+  (SmtLibSemantics.smtLibRoundMethod eout sout SmtLibSemantics.smtLibV SmtLibSemantics.smtLibV).roundRTZ sign
+    (ExtRat.NaN) = PackedFloat.mkNaN := by
+  simp [SmtLibSemantics.RoundMethod.roundRTZ]
+  rcases sign <;> simp
+
+
+@[simp]
+theorem round_eq_mkNaN_of_NaN {sign} {eout sout : Nat} {rm : RoundingMode} :
+    (SmtLibSemantics.smtLibRoundMethod eout sout SmtLibSemantics.smtLibV SmtLibSemantics.smtLibV).round
+        rm sign ExtRat.NaN = PackedFloat.mkNaN := by
+  rcases rm
+  · simp
+  · simp
+  · simp
+  · simp
+  · simp
+
+@[simp]
+theorem round_eq_mkZero_of_mkZero {zeroSign : Bool} {eout sout : Nat} {rm : RoundingMode} :
+    (SmtLibSemantics.smtLibRoundMethod eout sout SmtLibSemantics.smtLibV SmtLibSemantics.smtLibV).round
+        rm zeroSign (ExtRat.Number 0) = PackedFloat.getZero eout sout zeroSign := by
+  rcases rm <;> sorry
+
+theorem roundQ_Number_eq_round (er : ExtRat) (uf : UnpackedFloat ein sin)
+    (hruf : ExtRat.Number uf.toRat = er) :
+    (SmtLibSemantics.smtLibRoundMethod eout sout SmtLibSemantics.smtLibV SmtLibSemantics.smtLibV).round rm sign
+      er =
+      (UnpackedFloat.round uf rm).pack := by sorry
+
+
+-- theorem roundQ_Number_eq_round (r : Rat) (uf : UnpackedFloat ein sin)
+--     (hruf : uf.toRat = r) :
+--     (SmtLibSemantics.smtLibRoundMethod eout sout SmtLibSemantics.smtLibV SmtLibSemantics.smtLibV).round rm sign
+--       (.Number r : ExtRat) =
+--       (UnpackedFloat.round uf rm).pack := by sorry
+
+
+-- theorem roundQ_eq_round_of_toExtRat_mkNumber :
+--     (SmtLibSemantics.smtLibRoundMethod eout sout SmtLibSemantics.smtLibV SmtLibSemantics.smtLibV).round rm sign
+--       (EUnpackedFloat.mkNumber inf).toExtRat =
+--       (UnpackedFloat.round inf rm).pack := by sorry
+
+@[simp]
+theorem roundQ_eq_round_of_Infinity {zeroSign infSign : Bool} {e s : Nat} {rm : RoundingMode} :
+    (SmtLibSemantics.smtLibRoundMethod e s SmtLibSemantics.smtLibV SmtLibSemantics.smtLibV).round rm zeroSign
+      (ExtRat.Infinity infSign) =
+      PackedFloat.getInfinity e s infSign := by sorry
+
+/--
+Case splitting on the different values a packed float
+can have: it can be nan, infinity, zero, or a nonzero normal/subnormal.+
+-/
+@[elab_as_elim]
+theorem PackedFloat.kindCasesNaNInfZeroNum {P : PackedFloat e s → Prop}
+    (x : PackedFloat e s)
+    (nanCase : ∀ (n : PackedFloat e s), n.isNaN → P n)
+    (infCase : ∀ sign, P (PackedFloat.getInfinity e s sign))
+    (zeroCase : ∀ sign, P (PackedFloat.getZero e s sign))
+    (numCase : ∀ (n : PackedFloat e s), n.isNormOrNonzeroSubnorm → P n) :
+    P x := by
+  have := x.classification_exhaustive
+  simp at this
+  by_cases h1 : x.isNaN
+  · grind
+  · by_cases h2 : x.isInfinite
+    · grind
+    · by_cases h3 : x.isZero
+      · grind
+      · by_cases h4 : x.isNonzeroSubnorm
+        · grind
+        · by_cases h5 : x.isNorm
+          · grind
+          · grind
+
+@[grind <=]
+theorem PackedFloat.eq_of_unpack_eq_unpack_of_isInfinity {x y : PackedFloat e s}
+    (hs : 0 < s) (he : 0 < e)
+    (hx : x.isInfinite) (hy : y.isInfinite) (h : x.unpack = y.unpack) :
+    x = y := by
+  cases x using PackedFloat.kindCasesNaNInfZeroNum <;> try grind
+
+/--
+Example theorem we will prove, using our proof strategy of proving against the SMT-Lib semantics.
+-/
+theorem mul_eq_mul {ein sin : Nat} (hsin : 0 < sin) (he : 0 < ein)
+    (eout sout : Nat) (rm : RoundingMode) (a b : PackedFloat ein sin) :
+    Fp.SmtLibSemantics.SmtLibFunctions.mul (Fp.SmtLibSemanticsQ.smtLibRoundMethodQ ein sin)
+    rm a b = PackedFloat.mul rm a b := by
+  simp [SmtLibSemantics.SmtLibFunctions.mul]
+  rw [PackedFloat.mul, EUnpackedFloat.mul]
+  cases a using PackedFloat.kindCasesNaNInfZeroNum
+  case nanCase hnan =>
+    simp [hnan]
+    rw [round_eq_mkNaN_of_NaN]
+  case infCase signa =>
+    simp [hsin]
+    rw [← ExtRat.mul_def]
+    unfold ExtRat.mul
+    simp
+    cases b using PackedFloat.kindCasesNaNInfZeroNum
+    case nanCase hb =>
+      simp [hb]
+      -- | why does this not apply automatically?
+      rw [round_eq_mkNaN_of_NaN]
+    case infCase signb =>
+      simp [hsin]
+      rw [roundQ_eq_round_of_Infinity] -- TODO: this should just 'simp'
+    case zeroCase signb =>
+      simp [he]
+      rw [round_eq_mkNaN_of_NaN] -- TODO: this probably suffers due to TC instantiation :(
+    case numCase hb =>
+      -- TODO: prove a theorem that says that 'isNumber -> ∃ r such that b.toExtRat' = Number r'.
+      -- Use that to simplify the value.
+      -- simp [he, hsin]
+      -- | I want this to automatically apply with simp?
+      -- rw [PackedFloat.unpack_eq_mkNumber_of_isNormOrNonzeroSubnorm hb]
+      -- rw [<- PackedFloat.toExtRat_eq_toExtRat']
+      -- rw [← PackedFloat.toExtRat_unpack_eq_toExtRat]
+      rw [b.toExtRat'_eq_Number_of_isNormOrNonzeroSubnorm hb]
+      simp [b.toNumberRat_ne_zero hb]
+      simp [show ¬ b.isNaN by grind]
+      simp [show ¬ b.isZero by grind]
+      rw [roundQ_eq_round_of_Infinity]
+      congr
+      rw [b.unpack_eq_mkNumber_of_isNormOrNonzeroSubnorm hb]
+      simp only [EUnpackedFloat.num_mkNumber, PackedFloat.sign_unpackNormOrNonzeroSubnorm_eq_sign]
+      -- ⊢ decide (b.toNumberRat < 0) = b.unpack.num.sign
+      sorry
+  case zeroCase sign =>
+    simp [he]
+    cases b using PackedFloat.kindCasesNaNInfZeroNum
+    case nanCase hb =>
+      simp [hb]
+      rw [round_eq_mkNaN_of_NaN]
+    case infCase signb =>
+      simp [hsin]
+      rw [round_eq_mkNaN_of_NaN] -- TODO: this probably suffers due to TC instantiation :(
+    case zeroCase signb =>
+      simp [he]
+      rw [round_eq_mkZero_of_mkZero]
+      simp [SmtLibSemantics.SmtLibFunctions.xorSign]
+      simp [show decide (ein = 0) = false by grind]
+    case numCase hb =>
+      rw [PackedFloat.unpack_eq_mkNumber_of_isNormOrNonzeroSubnorm hb]
+      simp
+      rw [PackedFloat.toExtRat'_eq_Number_of_isNormOrNonzeroSubnorm hb]
+      simp
+      rw [round_eq_mkZero_of_mkZero]
+      simp [SmtLibSemantics.SmtLibFunctions.xorSign]
+      simp [show ¬ b.isNaN by grind]
+      simp [show ¬ b.isInfinite by grind]
+      -- TODO: prove a theorem that says that 'isNumber -> ∃ r such that b.toExtRat' = Number r'.
+      -- Use that to simplify the value.
+  case numCase ha =>
+    rw [PackedFloat.unpack_eq_mkNumber_of_isNormOrNonzeroSubnorm ha]
+    rw [PackedFloat.toExtRat'_eq_Number_of_isNormOrNonzeroSubnorm ha]
+    -- interesting case, when a is a number.
+    cases b using PackedFloat.kindCasesNaNInfZeroNum
+    case nanCase hb =>
+      simp [hb]
+      rw [round_eq_mkNaN_of_NaN]
+    case infCase signb =>
+      simp [hsin]
+      have : ¬ a.isZero := by grind
+      simp [this]
+      rw [← ExtRat.mul_def, ExtRat.mul]
+      simp only [SmtLibSemantics.instExtendedRat, SmtLibSemantics.instExtendedRat.eq_1, roundQ_eq]
+      simp [show a.toNumberRat < 0 ↔ a.sign = true by sorry]
+      simp [show a.toNumberRat = 0 ↔ a.isZero by sorry]
+      simp [show ¬ a.isZero by grind]
+      rw [roundQ_eq_round_of_Infinity]
+      grind
+    case zeroCase signb =>
+      simp [he]
+      rw [round_eq_mkZero_of_mkZero]
+      simp [SmtLibSemantics.SmtLibFunctions.xorSign]
+    case numCase hb =>
+      rw [PackedFloat.unpack_eq_mkNumber_of_isNormOrNonzeroSubnorm hb]
+      simp
+      have : ¬ a.isZero := by grind
+      simp [this]
+      have : ¬ b.isZero := by grind
+      simp [this]
+      rw [roundQ_Number_eq_round]
+      rw [PackedFloat.toExtRat'_eq_Number_of_isNormOrNonzeroSubnorm hb]
+      simp only [ExtRat.number_mul_number_eq, ExtRat.Number.injEq]
+      -- Purely arithmetic statement.
+      -- ⊢ (a.unpackNormOrNonzeroSubnorm.mul b.unpackNormOrNonzeroSubnorm).toRat = a.toNumberRat * b.toNumberRat
+      sorry
+end Fp
