README.md
@@ -26,7 +26,6 @@ We would appreciate pull requests that improve our testing.
 We audited several librares, but settled on our choices since they enable us to
 test all rounding modes for small bitwidths.
 
-- [SMT-LIB floating point specification](https://smt-lib.org/theories-FloatingPoint.shtml).
 - [Berlekee TestFloat](https://www.jhauser.us/arithmetic/TestFloat.html).
 - [Ulp plots](https://blogs.mathworks.com/cleve/2017/01/23/ulps-plots-reveal-math-function-accurary/).
 _ [Kahan Floating Point Paranoia](https://people.math.sc.edu/Burkardt/c_src/paranoia/paranoia.c).
@@ -36,5 +35,8 @@ _ [Kahan Floating Point Paranoia](https://people.math.sc.edu/Burkardt/c_src/para
 
 #### References
 
+- [IEEE 754-2008 spec](https://ieeexplore.ieee.org/stamp/stamp.jsp?tp=&arnumber=4610935)
+- [SMT-LIB floating point specification](https://smt-lib.org/theories-FloatingPoint.shtml).
+- [BTRW15: An Automatable Formal Semantics for IEEE 754](https://smt-lib.org/papers/BTRW15.pdf)
 - [2020-2021 Floating Point Course @ Cambridge](https://www.cl.cam.ac.uk/teaching/1011/FPComp/)
 - [Numerical Computing with IEEE Floating Point Arithmetic by Michael L. Overton.](https://dl.acm.org/doi/pdf/10.1145/103162.103163)
